finished compression

theories/FOLP/Compression_const.v
@@ -3,32 +3,58 @@
 Require Import Equations.Equations Fin.
 From Undecidability.FOLP Require Export FullTarski.
 
+
+
+(* Prelim (to be moved) *)
+
+Lemma cast_refl X n (v : vector X n) :
+  cast v eq_refl = v.
+Proof.
+  induction v; cbn; congruence.
+Qed.
+
+
+
+(* Satisfiability (not yet classical) *)
+
+Definition SAT Sigma (phi : @form Sigma) :=
+  exists D (I : @interp Sigma D) rho, rho ⊨ phi.
+
+
+
+(* STEP 1: compression into a single relation symbol *)
+
 Section Compression.
 
   Context { Sigma : Signature }.
 
-  Notation fin := Fin.t.
+  (* Input: signature only containing relations of a fixed arity *)
 
   Variable arity : nat.
   Hypothesis arity_const : forall P, pred_ar P = arity.
+  Hypothesis funcs_empty : Funcs -> False.
+
+  (* Output: signature with constants for each relation and a single relation *)
 
   Definition compress_sig :=
-    {| Funcs := Funcs + Preds;
-       fun_ar := fun f => match f with inl f => fun_ar f | _ => 0 end;
+    {| Funcs := Preds;
+       fun_ar := fun _ => 0;
        Preds := unit;
        pred_ar := fun _ => S arity |}.
+
+  (* Conversion: each atom P_i(x, y, ...) is replaced by P (i, x, y, ...) *)
 
   Fixpoint convert_t (t : @term Sigma) : @term compress_sig :=
     match t with
     | var_term s => var_term s
-    | Func f v => @Func compress_sig (inl f) (Vector.map convert_t v)
+    | Func f v => False_rect _ (funcs_empty f)
     end.
 
   Definition convert_v n (v : vector term n) :=
     Vector.map convert_t v.
   
   Definition encode_v P (v : vector term (pred_ar P)) :=
-    Vector.cons (@Func compress_sig (inr P) Vector.nil) (cast (convert_v v) (arity_const P)).
+    Vector.cons (@Func compress_sig P Vector.nil) (cast (convert_v v) (arity_const P)).
 
   Fixpoint encode (phi : @form Sigma) : @form compress_sig :=
     match phi with
@@ -41,8 +67,7 @@ Section Compression.
     | All phi => All (encode phi)
     end.
 
-  
-
+  (* Direction 1: sat phi -> sat (encode phi) *)
 
   Section to_compr.
 
@@ -67,9 +92,7 @@ Section Compression.
       @interp compress_sig (D + Preds).
     Proof.
       split.
-      - intros [f|P] v.
-        + left. exact (@i_f _ _ I f (vec_fill v)).
-        + right. exact P.
+      - intros P v. right. exact P.
       - intros [] v; cbn in *.
         destruct (Vector.hd v) as [d|P].
         + exact True.
@@ -82,54 +105,23 @@ Section Compression.
     Lemma eval_to_compr (rho : nat -> D) t :
       inl (eval rho t) = eval (convert_env rho) (convert_t t).
     Proof.
-      induction t using strong_term_ind; cbn; trivial. repeat f_equal.
-      induction v; cbn; trivial. rewrite <- H, IHv; intuition.
-    Qed.
-
-    Lemma cast_refl X n (v : vector X n) :
-      cast v eq_refl = v.
-    Proof.
-      induction v; cbn; congruence.
+      destruct t as [x | f v]; trivial.
+      exfalso. apply (funcs_empty f).
     Qed.
 
     Definition env_fill (rho : nat -> D + Preds) : nat -> D + Preds :=
       fun n => match (rho n) with inl d => inl d | inr P => inl d0 end.
 
-    Lemma env_fill_eval rho t :
-      eval (env_fill rho) (convert_t t) = eval rho (convert_t t).
-    Proof.
-      induction t using strong_term_ind; cbn; trivial.
-    Abort.
-
     Lemma env_fill_sat rho phi :
-      sat (env_fill rho) phi <-> sat rho phi.
-    Proof.
-      induction phi in rho |- *; try tauto.
-      - destruct P. cbn. admit.
-      - firstorder.
-      - firstorder.
-      - firstorder.
-      - split; intros H d.
-        + apply IHphi. destruct d; eapply sat_ext; try apply H; now destruct x.
-        + apply IHphi. destruct d; eapply sat_ext; try apply IHphi, H; destruct x; try reflexivity.
-          all: unfold env_fill; cbn; now destruct (rho x).
-      - split; intros [d H].
-        + exists d. apply IHphi. apply IHphi in H. destruct d; eapply sat_ext; try apply H; destruct x; try reflexivity.
-          all: unfold env_fill; cbn; now destruct (rho x).
-        + exists d. apply IHphi. apply IHphi in H. destruct d; eapply sat_ext; try apply H; destruct x; try reflexivity.
-          all: unfold env_fill; cbn; now destruct (rho x).
-    Admitted.
-
-    Lemma env_fill_sat' rho phi :
       sat (env_fill rho) (encode phi) <-> sat rho (encode phi).
     Proof.
       induction phi in rho |- *; try tauto.
       - cbn. rewrite <- (arity_const P), !cast_refl.
         replace (vec_fill (Vector.map (eval (env_fill rho)) (convert_v t)))
                 with (vec_fill (Vector.map (eval rho) (convert_v t))); try reflexivity.
-        induction t; cbn; trivial. rewrite IHt. destruct h; cbn. 
+        induction t; cbn; trivial. rewrite IHt. destruct h as [x | f v]; cbn. 
         + unfold env_fill. now destruct rho.
-        
+        + exfalso. apply (funcs_empty f).
       - firstorder.
       - firstorder.
       - firstorder.
@@ -142,7 +134,7 @@ Section Compression.
           all: unfold env_fill; cbn; now destruct (rho x).
         + exists d. apply IHphi. apply IHphi in H. destruct d; eapply sat_ext; try apply H; destruct x; try reflexivity.
           all: unfold env_fill; cbn; now destruct (rho x).
-    Admitted.
+    Qed.
 
     Lemma sat_to_compr (rho : nat -> D) phi :
       sat rho phi <-> sat (convert_env rho) (encode phi).
@@ -168,26 +160,28 @@ Section Compression.
 
   End to_compr.
 
+  (* Direction 2: sat (encode phi) -> sat phi *)
+
   Section from_compr.
 
     Context { D : Type }.
     Context { I : @interp compress_sig D }.
 
-    Notation index P := (@i_f _ _ I (inr P) Vector.nil).
+    Notation index P := (@i_f _ _ I P Vector.nil).
 
     Local Instance uncompr_interp :
       @interp Sigma D.
     Proof.
       split.
-      - intros f v. exact (@i_f _ _ I (inl f) v).
+      - intros f v. exfalso. apply (funcs_empty f).
       - intros P v. exact (@i_P _ _ I tt (Vector.cons (index P) (cast v (arity_const P)))).
     Defined.
 
-    Lemma eval_from_compr (rho : nat -> D) t :
+    Lemma eval_from_compr (rho : nat -> D) (t : @term Sigma) :
       eval rho t = eval rho (convert_t t).
     Proof.
-      induction t using strong_term_ind; cbn; trivial.
-      f_equal. erewrite vec_comp. apply vec_map_ext. apply H. reflexivity.
+      destruct t as [x | f v]; trivial.
+      exfalso. apply (funcs_empty f).
     Qed.
 
     Lemma sat_from_compr (rho : nat -> D) phi :
@@ -201,5 +195,15 @@ Section Compression.
     Qed.
 
   End from_compr.
+
+  (* Main result *)
+
+  Theorem sat_compr (phi : @form Sigma) :
+    SAT phi <-> SAT (encode phi).
+  Proof.
+    split; intros (D & I & rho & H).
+    - exists _, (compr_interp (rho 0)), (convert_env rho). now apply sat_to_compr.
+    - exists _, uncompr_interp, rho. now apply sat_from_compr.
+  Qed.
 
 End Compression.
